theories/prob_eff_lang/probblaze/examples/DH_KE/s_channel.v
@@ -1,5 +1,5 @@
 From clutch.prob_eff_lang.probblaze Require Export notation valgroup.
-From clutch.prob_eff_lang.probblaze Require Import definition.
+From clutch.prob_eff_lang.probblaze Require Export definition.
 
 Import fingroup.
 
@@ -8,12 +8,10 @@ Import fingroup.fingroup.
 Import valgroup_notation.
 Import valgroup_tactics.
 
-
-Section secure_channel.
+Section sec_channel.
   Context {vg : val_group}.
   Context {cg : clutch_group_struct}.
   Context {vgg : @val_group_generator vg}.
-
 
   #[local] Notation n := (S n'').
 
@@ -21,7 +19,7 @@ Section secure_channel.
   Definition RecvSecure (e : expr) := InjR e.
 
   (*In this implementation, we are not parametrizing by the party*)
-  (*ONE-SHOT authenticated channel ideal functionality*)
+  (*Unidirectional channel ideal functionality for sending ONE message *)
   Definition F_OAUTH (channel : label) f : expr :=
      let: "message" := ref NONEV in
      handle: f with
@@ -46,13 +44,12 @@ Section secure_channel.
      | return "y" => #()%V
     end.
 
-
+            
   (*placeholder for now *)
   Definition xor (e1 e2 : expr) : expr := #()%V.  
 
-  
-  (*ONE-SHOT Secure channel functionality
-   Assumes a fix direction of sending the message, from Alice to Bob*)
+  (*ONE message unidirectional secure channel functionality.
+    Assume a fixed direction of sending the message, from Alice to Bob *)
   Definition CHAN (getKey channel : label) f : expr :=
     let: "message" := ref NONEV in
     handle: f with
@@ -64,166 +61,131 @@ Section secure_channel.
             match: !"message" with
             | NONE => "message" <- SOME "m";;
                      let: "key" := do: getKey ("dst") in
-                                              match: "key" with
-                                                (*is this correct?*)
-                                              | NONE => "k" NONEV
-                                              | SOME "x" =>
-                                                  let: "enc_m" := xor "x" "m" in
-                                                  (do: channel (Send ("enc_m", bob)));; "k" #()%V
-                                              end    
+                                     match: "key" with
+                                     | NONE => "k" NONEV
+                                     | SOME "x" =>
+                                         let: "enc_m" := xor "x" "m" in
+                                         (do: channel (Send ("enc_m", bob)));;
+                                         "k" #()%V
+                                     end
+                                       
             | SOME "message" => "k" NONEV
             end
-            (*match: "dst" with
-            (*Alice *)
-            | InjL <> => match: !"message" with
-                       | NONE => "message" <- SOME "m";;
-                                let: "key" := do: "getKey" ("dst") in
-                                              match: "key" with
-                                                (*is this correct?*)
-                                              | NONE => "k" NONEV
-                                              | SOME "x" =>
-                                                  let: "enc_m" := xor "x" "m" in
-                                                  (do: channel (Send ("enc_m", bob)));; "k" #()%V
-                                              end    
-                        | SOME "message" => "k" NONEV (*is this correct? *)
-                      end                              
-         (*Bob*)                        
-             | InjR <> => match: !"message" with
-                       | NONE => "message" <- SOME "m";;
-                                let: "key" := do: "getKey" ("dst") in
-                                              match: "key" with
-                                                (*is this correct?*)
-                                              | NONE => "k" NONEV
-                                              | SOME "x" =>
-                                                  let: "enc_m" := xor "x" "m" in
-                                                  (do: channel (Send ("enc_m", alice)));; "k" #()%V
-                                              end
-                      | SOME "message" => "k" NONEV (*is this correct? *)
-                      end                                                           
-            end*)
-              
-            (*ReceiveSecure*)
-                                            |InjR "from" =>
-                                               let: "key" := do: getKey ("from") in
-                                                             match: "key" with
-                                                               (*is this correct?*)
-                                                             | NONE => "k" NONEV
-                                                             | SOME "x" =>
-                                                                 let: "r" := (do: channel (Recv "from")) in
-                                                                 match: "r" with
-                                                                 | NONE => "k" NONEV
-                                                                 | SOME "x'" =>
-                                                                     let: "enc_m" := xor "x" "x'" in
-                                                                     "k" (SOME "enc_m")
-                                                                 end
-                                                              end                
-                                               
-                                               
+          (*RecvSecure*)
+        | InjR "from" =>
+            let: "key" := do: getKey ("from") in
+                            match: "key" with
+                            | NONE => "k" NONEV
+                            | SOME "key" =>
+                                let: "r" := (do: channel (Recv "from")) in
+                                match: "r" with
+                                | NONE => "k" NONEV
+                                | SOME "x" =>
+                                    let: "enc_m" := xor "key" "x" in
+                                    "k" (SOME "enc_m")
+                                end       
+                            end                              
         end
-    | return "y" => #()%V end.
+    | return "y" => #()%V
+  end.
   
-
-
-  
-  (* Ideal functionality of the ONE-SHOT secure channel*)
+                                           
+  (* Ideal functionality of the ONE-SHOT secure channel *)
   Definition F_CHAN (channel : label) f : expr :=
     let: "message" := ref NONEV in
     handle: f with
     | effect channel "payload", rec "k" as multi =>
         match: "payload" with
-        (*SendSecure *)
+          (*SendSecure*)
         | InjL "payload" =>
             let, ("m", "dst") := "payload" in
             match: !"message" with
             | NONE => "message" <- SOME "m";;
                      (do: channel (Send (#0, "dst")));;
-                     "k" #()%V
+                     "k" #()%V 
             | SOME "x" => "k" #()%V
             end
-        (*ReceiveSecure*)
-        |InjR "from" =>
-           let: "r" := (do: channel (Recv "from")) in
-           match: "r" with
-           | NONE => "k" NONEV
-           | SOME "x" => "k" !"message"
-           end
+          (*ReceiveSecure*)
+        | InjR "from" =>
+            let: "r" := (do: channel (Recv "from")) in
+            match: "r" with
+            | NONE => "k" NONEV
+            | SOME "x" => "k" !"message"
+            end              
         end
-              
-    | return "y" => #()%V end.
-  
-    
-   Definition CHAN_SIM (channel : label) (f : expr) : expr :=
-      let: "α" := alloc #n in 
-      let: "message" := ref NONEV in      
+    | return "y" => #()%V
+    end.
+                        
+ (*Simulator for the one message secure channel *)
+ (* Assumes a fixed direction from Alice to Bob *)       
+  Definition CHAN_SIM (channel leak : label) (f : expr) : expr :=
+    let: "α" := alloc #n in
+    let: "message" := ref NONEV in
     handle: f with
     | effect channel "payload", rec "k" as multi =>
         match: "payload" with
-          (*Leak effect for sending a message *)
-        | InjL "payload" => 
+          (*Broadcast a message*)
+        | InjL "payload" =>
+            (* assuming "dst" is alice for now *)
             let, ("m", "dst") := "payload" in
-            (do: channel (Send (#0, alice)));;
-                let: "r" := do: channel (Recv bob) in
-                              match: "r" with
-                              | NONE => "k" NONE
-                              | SOME "x" =>
-                                  let: "m" :=
-                                    (match: !"message" with
-                                     | NONE =>
-                                         let:
-                                           "m":= (samplelbl "α" #()%V) in "message" <- SOME "m";; "m"
-                                     | SOME "m" => "m"
-                                     end) in
-                                  let: "mA" := g^"m" in
-                                  (do: channel (Send ("mA", alice)));;
-                                  "k" #()%V
-                              end
-            (*match: "dst" with
-              (*Alice *)
-             | InjL <> =>
-                (do: channel (Send (#0, alice)));;
-                let: "r" := do: channel (Recv bob) in
-                              match: "r" with
-                              | NONE => "k" NONE
-                              | SOME "x" =>
-                                  let: "m" :=
-                                    (match: !"message" with
-                                     | NONE =>
-                                         let:
-                                           "m":= (samplelbl "α" #()%V) in "message" <- SOME "m";; "m"
-                                     | SOME "m" => "m"
-                                     end) in
-                                  let: "mA" := g^"m" in
-                                  (do: channel (Send ("mA", alice)));;
-                                  "k" #()%V
-                              end                                   
-               (*Bob*)
-             | InjR <> =>
-                (do: channel (Send (#0, bob)));;
-                let: "r" := do: channel (Recv alice) in
-                              match: "r" with
-                              | NONE => "k" NONE
-                              | SOME "x" =>
-                                  let: "m" :=
-                                    (match: !"message" with
-                                     | NONE =>
-                                         let:
-                                           "m":= (samplelbl "β" #()%V) in "message" <- SOME "m";; "m"
-                                     | SOME "m" => "m"
-                                     end) in
-                                  let: "mB" := g^"m" in
-                                  (do: channel (Send ("mB", bob)));;
-                                  "k" #()%V
-                              end                      
-            end*)
-          (*Leak effect for receiving a message *)
-         | InjR "from" =>
-            let: "r" := do: channel (Recv "from") in
-                         match: "r" with
+            (do: leak ("dst"));;
+            let: "r" := do: channel (Recv bob) in
+                          match: "r" with
                           | NONE => "k" NONE
-                          | SOME "x" => "k" (SOME #0)
-                         end
+                          | SOME "x" =>
+                              let: "m" :=
+                                (match: !"message" with
+                                     | NONE =>
+                                         let:
+                                           "m":= (samplelbl "α" #()%V) in "message" <- SOME "m";; "m"
+                                     | SOME "m" => "m"
+                                     end) in
+                              let: "mA" := g^"m" in
+                              (do: channel (Send ("mA", alice)));;
+                              "k" #()%V
+                          end
+                            
+         | InjR "from " =>
+             let: "r" := do: channel (Recv "from") in
+                           match: "r" with
+                           | NONE => "k" NONE
+                           | SOME "x" =>
+                               (do: leak ("from"));;
+                               "k" (SOME #0)
+                           end                             
         end
     | return "y" => "y" end.
 
-                          
-End secure_channel.
+
+    Definition F_KE_L (getKey channel leak : label) f : expr :=
+    (* Magically share a presampled key *)
+    let: "c" := (sample #()%V) in
+    let: "key" := g ^ "c" in
+
+    handle: f with
+    | effect getKey "p", rec "k" as multi =>
+        match: "p" with
+          (* Alice *)
+          InjL <> =>
+            (* Send a dummy value *)
+            (do: leak (bob));;
+            (* Receive a dummy value *)
+            let: "r" := do: channel Recv bob in
+            match: "r" with
+              NONE => "k" NONEV
+            | SOME "w" => "k" (SOME "key")
+            end
+        (* Bob  *)
+        | InjR <> =>
+            let: "r" := do: channel Recv alice in
+            match: "r" with
+              NONE => "k" NONEV
+            | SOME "w" => 
+                (do: leak (alice));;
+                "k" (SOME "key")
+            end
+       end
+    | return "y" => "y" end.
+
+
+End sec_channel.
